crates/sui/src/sui_move/sui-natives.bpl
@@ -13,26 +13,29 @@ axiom $ADRESS_LENGTH == 20;
 
 // helper procedure with hard-coded length of vevtor for converting vector to int. 
 // TODO: This is a temporary solution.
-procedure {:inline 1} $2_address_deserialize(bytes: Vec (int)) returns (res: int)
+function $2_peel_vector_to_address(bytes: Vec (int), len: int): int
 {
-    var index, addr: int;
-    index, addr := 0, 0;
-
-    while (index < $ADRESS_LENGTH)
-    {
-        addr := addr * 256 + ReadVec(bytes, index);
-        index := index + 1;
-    }
-    res := addr;
-    return;
-    // (((((((((((((((((((ReadVec(bytes, 0) * 256 + ReadVec(bytes, 1)) * 256 + ReadVec(bytes, 2)) * 256 + ReadVec(bytes, 3)) * 256 + ReadVec(bytes, 4)) * 256 + ReadVec(bytes, 5)) * 256 + ReadVec(bytes, 6)) * 256 + ReadVec(bytes, 7)) * 256 + ReadVec(bytes, 8)) * 256 + ReadVec(bytes, 9)) * 256 + ReadVec(bytes, 10)) * 256 + ReadVec(bytes, 11)) * 256 + ReadVec(bytes, 12)) * 256 + ReadVec(bytes, 13)) * 256 + ReadVec(bytes, 14)) * 256 + ReadVec(bytes, 15)) * 256 + ReadVec(bytes, 16)) * 256 + ReadVec(bytes, 17)) * 256 + ReadVec(bytes, 18)) * 256 + ReadVec(bytes, 19))
+    if len > 0 then 256 * $2_peel_vector_to_address(bytes, len-1) + ReadVec(bytes, len-1)
+    else 0
 }
+    // addr := 0;
+    // var i: int;
+    // i := 0;
+    // while (i < $ADRESS_LENGTH)
+    // {
+    //     addr := addr * 256 + ReadVec(bytes, i);
+    //     i := i + 1;
+    // }
+    // addr
 
-axiom (forall v1, v2: Vec (int) :: {$2_address_deserialize(v1), $2_address_deserialize(v2)}
-   $IsEqual'vec'u8''(v1, v2) <==> $IsEqual'address'($2_address_deserialize(v1), $2_address_deserialize(v2)));
+    // (((((((((((((((((((ReadVec(bytes, 0) * 256 + ReadVec(bytes, 1)) * 256 + ReadVec(bytes, 2)) * 256 + ReadVec(bytes, 3)) * 256 + ReadVec(bytes, 4)) * 256 + ReadVec(bytes, 5)) * 256 + ReadVec(bytes, 6)) * 256 + ReadVec(bytes, 7)) * 256 + ReadVec(bytes, 8)) * 256 + ReadVec(bytes, 9)) * 256 + ReadVec(bytes, 10)) * 256 + ReadVec(bytes, 11)) * 256 + ReadVec(bytes, 12)) * 256 + ReadVec(bytes, 13)) * 256 + ReadVec(bytes, 14)) * 256 + ReadVec(bytes, 15)) * 256 + ReadVec(bytes, 16)) * 256 + ReadVec(bytes, 17)) * 256 + ReadVec(bytes, 18)) * 256 + ReadVec(bytes, 19))
+// }
 
-axiom (forall v: Vec (int) :: {$2_address_deserialize(v)}
-     ( var r := $2_address_deserialize(v); $IsValid'address'(r) ));
+axiom (forall v1, v2: Vec (int) :: {$2_peel_vector_to_address(v1, $ADRESS_LENGTH), $2_peel_vector_to_address(v2, $ADRESS_LENGTH)}
+   $IsEqual'vec'u8''(v1, v2) <==> $IsEqual'address'($2_peel_vector_to_address(v1, $ADRESS_LENGTH), $2_peel_vector_to_address(v2, $ADRESS_LENGTH)));
+
+axiom (forall v: Vec (int) :: {$2_peel_vector_to_address(v, $ADRESS_LENGTH)}
+     ( var r := $2_peel_vector_to_address(v, $ADRESS_LENGTH); $IsValid'address'(r) ));
 
 procedure {:inline 1} $2_address_from_bytes(bytes: Vec (int)) returns (res: int)
 {
@@ -42,18 +45,11 @@ procedure {:inline 1} $2_address_from_bytes(bytes: Vec (int)) returns (res: int)
         call $ExecFailureAbort();
         return;
     }
-    call res := $2_address_deserialize(bytes);
+    res := $2_peel_vector_to_address(bytes, $ADRESS_LENGTH);
 }
 
-procedure {:inline 1} $2_address_$from_bytes(bytes: Vec (int)) returns (res: int)
-{
-    var len: int;
-    len := LenVec(bytes);
-    if (len != 20) {
-        call $ExecFailureAbort();
-        return;
-    }
-    call res := $2_address_deserialize(bytes);
+function {:inline} $2_address_$from_bytes(bytes: Vec (int)): int {
+    $2_peel_vector_to_address(bytes, $ADRESS_LENGTH)
 }
 
 function $2_u256_from_address(addr: int): int
